@prefix : <https://open-manufacturing.org/ontologies/I4.0/Equipment/> .
@prefix owl: <http://www.w3.org/2002/07/owl#> .
@prefix rdf: <http://www.w3.org/1999/02/22-rdf-syntax-ns#> .
@prefix xml: <http://www.w3.org/XML/1998/namespace> .
@prefix xsd: <http://www.w3.org/2001/XMLSchema#> .
@prefix rdfs: <http://www.w3.org/2000/01/rdf-schema#> .
@prefix dc: <http://purl.org/dc/elements/1.1/> .
@base <https://open-manufacturing.org/ontologies/I4.0/Equipment/> .

<https://open-manufacturing.org/ontologies/I4.0/Equipment> rdf:type owl:Ontology ;
                                                                dc:contributor "https://www.linkedin.com/in/ram-sashank-dinavahi-123296a0/" ;
                                                                dc:created "April 27th, 2022"@en ;
                                                                dc:creator "Piotr Janik (Intel), Denis Molin (Tera Data), Soufiane Ameziane (Tera Data)"@en ,
                                                                                                          "https://www.linkedin.com/in/dr-felix-l%C3%B6sch-0083294b/" ,
                                                                                                          "https://www.linkedin.com/in/dr-irlan-grangel-gonzalez/" ,
                                                                                                          "https://www.linkedin.com/in/fabio-massari-b63892/" ,
                                                                                                          "https://www.linkedin.com/in/marcel-keller-5591a174/" ,
                                                                                                          "https://www.linkedin.com/in/nico-wilhelm-5b306867/" ;
                                                                dc:modified "June 22nd, 2022"@en ;
                                                                dc:title "OMP I4.0 Core Information Model - Equipment Ontology"@en ;
                                                                rdfs:comment "This ontology models concepts and relationships to organize assets according to logical principles"@en ;
                                                                rdfs:label "OMP I4.0 Core Information Model - Equipment Ontology"@en ;
                                                                owl:versionInfo "1.0"@en .


#################################################################
#    Object Properties
#################################################################

###  https://open-manufacturing.org/ontologies/I4.0/Equipment/belongsToLine
:belongsToLine rdf:type owl:ObjectProperty ;
               rdfs:subPropertyOf owl:topObjectProperty ;
               rdfs:domain :Station ;
               rdfs:range :Line ;
               rdfs:label "belongs to line"@en .


###  https://open-manufacturing.org/ontologies/I4.0/Equipment/belongsToPlant
:belongsToPlant rdf:type owl:ObjectProperty ;
                rdfs:subPropertyOf owl:topObjectProperty ;
                rdfs:domain :WorkCenter ;
                rdfs:range :Plant ;
                rdfs:comment "Relationship between \"WorkCenter\" and \"Plant\""@en ;
                rdfs:label "belongs to plant"@en .


###  https://open-manufacturing.org/ontologies/I4.0/Equipment/belongsToStation
:belongsToStation rdf:type owl:ObjectProperty ;
                  rdfs:subPropertyOf owl:topObjectProperty ;
                  rdfs:domain :WorkCell ;
                  rdfs:range :Station ;
                  rdfs:comment "Relationship between \"WorkCell\" and \"Station\""@en ;
                  rdfs:label "belongs to station"@en .


###  https://open-manufacturing.org/ontologies/I4.0/Equipment/belongsToWorkCenter
:belongsToWorkCenter rdf:type owl:ObjectProperty ;
                     rdfs:subPropertyOf owl:topObjectProperty ;
                     rdfs:domain :WorkUnit ;
                     rdfs:range :WorkCenter ;
                     rdfs:comment "Relationship between \"WorkUnit\" and \"WorkCenter\""@en ;
                     rdfs:label "belongs to work center"@en .


###  https://open-manufacturing.org/ontologies/I4.0/Equipment/consistsOfStation
:consistsOfStation rdf:type owl:ObjectProperty ;
                   rdfs:subPropertyOf owl:topObjectProperty ;
                   rdfs:domain :Line ;
                   rdfs:range :Station ;
                   rdfs:comment "Relationship between \"Line\" and \"Station\""@en ;
                   rdfs:label "consists of station"@en .


###  https://open-manufacturing.org/ontologies/I4.0/Equipment/consistsOfWorkCell
:consistsOfWorkCell rdf:type owl:ObjectProperty ;
                    rdfs:subPropertyOf owl:topObjectProperty ;
                    rdfs:domain :Station ;
                    rdfs:range :WorkCell ;
                    rdfs:comment "Relationship between \"Station\" and \"WorkCell\""@en ;
                    rdfs:label "consists of work cell"@en .


###  https://open-manufacturing.org/ontologies/I4.0/Equipment/consistsOfWorkCenter
:consistsOfWorkCenter rdf:type owl:ObjectProperty ;
                      rdfs:subPropertyOf owl:topObjectProperty ;
                      rdfs:domain :Plant ;
                      rdfs:range :WorkCenter ;
                      rdfs:comment "Relationship between \"Plant\" and \"WorkCenter\""@en ;
                      rdfs:label "consists of work center"@en .


###  https://open-manufacturing.org/ontologies/I4.0/Equipment/consistsOfWorkUnit
:consistsOfWorkUnit rdf:type owl:ObjectProperty ;
                    rdfs:subPropertyOf owl:topObjectProperty ;
                    rdfs:domain :WorkCenter ;
                    rdfs:range :WorkUnit ;
                    rdfs:comment "Relationship between \"WorkCenter\" and \"WorkUnit\""@en ;
                    rdfs:label "consists of work unit"@en .


###  https://open-manufacturing.org/ontologies/I4.0/Equipment/madeUpOfWorkUnit
:madeUpOfWorkUnit rdf:type owl:ObjectProperty ;
                  rdfs:subPropertyOf owl:topObjectProperty ;
                  rdfs:domain :WorkUnit ;
                  rdfs:range :WorkUnit ;
                  rdfs:comment "Transitive Relationship between \"WorkUnit\" with itself"@en ;
                  rdfs:label "made up of work unit"@en .


#################################################################
#    Classes
#################################################################

###  https://open-manufacturing.org/ontologies/I4.0/Equipment/Equipment
:Equipment rdf:type owl:Class ;
           rdfs:comment """Generalization for all logical elements required to organize or model your manufacturing hierarchy, sequence or flow.

Note 1: The formal UML role-based equipment model object is used to define the role-based equipment hierarchy information that is defined in IEC 62264-1.

Note 2: The model contains the information that may be used to construct the hierarchical models used in manufacturing scenarios.

Reference: IEC 62264-1, IEC 62264-2"""@en ;
           rdfs:label "Equipment"@en .


###  https://open-manufacturing.org/ontologies/I4.0/Equipment/Line
:Line rdf:type owl:Class ;
      rdfs:subClassOf :WorkCenter ;
      rdfs:comment """Collection of one or more sequentially ordered work units that work together to perform a defined sequence of production processes to manufacture or assemble a product that can be a final or a semi-finished product. 
A line is a subclass of a work center."""@en ;
      rdfs:label "Line"@en .


###  https://open-manufacturing.org/ontologies/I4.0/Equipment/Plant
:Plant rdf:type owl:Class ;
       rdfs:subClassOf :Equipment ;
       rdfs:comment "Complex and separate organizational structure set up. It is a logical grouping of a manufacturing entity. It contains other equipment such as work centers or work units. Plants may be part of business-oriented entities such as product lines, divisions, sales segments and so on."@en ;
       rdfs:label "Plant"@en .


###  https://open-manufacturing.org/ontologies/I4.0/Equipment/Pool
:Pool rdf:type owl:Class ;
      rdfs:subClassOf :WorkCenter ;
      rdfs:comment """Grouping of several parallel work units running the same process or sharing similar capabilities. 
A pool is a subclass of a work center."""@en ;
      rdfs:label "Pool"@en .


###  https://open-manufacturing.org/ontologies/I4.0/Equipment/Station
:Station rdf:type owl:Class ;
         rdfs:subClassOf :WorkUnit ;
         rdfs:comment """A logical grouping of equipment intended to produce a good. Stations are often are linked to a manufacturing process for a semi-finished or finished part. Subclass of a work unit. Stations belong to a line. A line can consist of 1..n stations.

One or more process segments may be linked to a station. 

Note 1: Assets or parts within an Asset represent a station well. Station can be linked to assets via the “isImplementedBy” relationship"""@en ;
         rdfs:label "Station"@en .


###  https://open-manufacturing.org/ontologies/I4.0/Equipment/WorkCell
:WorkCell rdf:type owl:Class ;
          rdfs:subClassOf :WorkUnit ;
          rdfs:comment """Logical sub groupings of stations. A station can consist of 1..n work cells. Subclass of a work unit.

Work cells are intended to implement a process segment. Usually, the mapping between process segment and work cell is a 1:1 mapping."""@en ;
          rdfs:label "Work Cell"@en .


###  https://open-manufacturing.org/ontologies/I4.0/Equipment/WorkCenter
:WorkCenter rdf:type owl:Class ;
            rdfs:subClassOf :Equipment ;
            rdfs:comment """Grouping of one or more work units or smaller work centers that are logically or geographically linked. Line and Pool are sub-classes of work centers. A work centers can consist of 1..n work centers (e.g., a pool is part of a line). 
This term does not refer to SAP work center. It is possible but not recommended to represent an asset as a work center."""@en ;
            rdfs:label "Work Center"@en .


###  https://open-manufacturing.org/ontologies/I4.0/Equipment/WorkUnit
:WorkUnit rdf:type owl:Class ;
          rdfs:subClassOf :Equipment ;
          rdfs:comment """Logical grouping of equipment at the level below a work center. A work unit can consist of smaller work units. A work unit logically represents the location of executing a manufacturing process and can be linked to a machine or machine component which physically executes the manufacturing process.

It performs production, storage, material movement, or any other Level three or level four scheduled activity according to the manufacturing operations and control systems hierarchy.

Reference: IEC 62264-1 ID:3.1.26"""@en ;
          rdfs:label "Work Unit"@en .


###  Generated by the OWL API (version 4.5.9.2019-02-01T07:24:44Z) https://github.com/owlcs/owlapi
